# 3진법 뒤집기

<br>

## 3진법 풀이법

<br>

## 풀이
```
import java.util.List;
import java.util.ArrayList;
import java.lang.Math;

class Solution {
    public int solution(int n) {
        List<Integer> terniaryList = new ArrayList<Integer>();
        int answer = 0;
        
        while (n != 0) {
            int remainder = n % 3;
            terniaryList.add(remainder);
            n = n / 3;
        }
        
        for (int i = 0; i < terniaryList.size(); i++) {
            int value = terniaryList.get(terniaryList.size() - i - 1) * (int)(Math.pow(3, i));
            answer += value;
        }
        
        return answer;
    }
}
```
